coq/lib/P4cub/Transformations/Lifting/LiftSpec.v
@@ -47,21 +47,19 @@ Section RelateExprDeclList.
 
   Polymorphic Hypothesis shift_exp_preserves_R : forall as1 as2 as3 a e,
       R (as1 ++ as3) e a ->
-      R (as1 ++ as2 ++ as3) (shift_exp (Shifter (length as1) (length as2)) e) a.
+      R (as1 ++ as2 ++ as3) (shift_exp (length as1) (length as2) e) a.
 
   Local Hint Constructors relate_decl_list : core.
   
   Polymorphic Lemma relate_decl_list_app : forall es1 es2 as1 as2,
       relate_decl_list R l es1 as1 ->
       relate_decl_list R l es2 as2 ->
-      relate_decl_list R l (shift_list shift_exp (Shifter 0 (length es1)) es2 ++ es1) (as2 ++ as1).
+      relate_decl_list R l (shift_list shift_exp 0 (length es1) es2 ++ es1) (as2 ++ as1).
   Proof using A R l shift_exp_preserves_R.
     intros es1 es2 as1 as2 h1 h2.
     generalize dependent as1.
     generalize dependent es1.
     induction h2; intros es1 as1 h1; cbn; auto.
-    unfold smother, RecordSet.set; cbn.
-    rewrite add_0_r.
     constructor; auto. rewrite <- app_assoc.
     rewrite (relate_decl_list_length _ _ _ _ h1).
     rewrite (relate_decl_list_length _ _ _ _ h2).
@@ -73,7 +71,7 @@ Section RelateExprDeclList.
   Polymorphic Lemma shift_pairs_relate_snd : forall ess ass,
       Forall2 (relate_decl_list R l) (map snd ess) ass ->
       relate_decl_list R l
-        (concat (map snd (shift_pairs shift_exp ess)))
+        (concat (snd (shift_pairs shift_exp ess)))
         (concat ass).
   Proof using A R l shift_exp_preserves_R.
     intros ess vss h.
@@ -81,15 +79,16 @@ Section RelateExprDeclList.
     generalize dependent ess.
     induction h; intros [| [e es] ess] hess; inv hess;
       unravel in *; auto.
-    pose proof IHh ess ltac:(auto) as ih; clear IHh.
-    rewrite map_snd_map, map_id.
-    assert (list_sum (map (length (A:=Exp.t)) (map snd ess))
-            = length (concat (map snd (shift_pairs shift_exp ess)))) as hlen.
-    { unfold list_sum.
-      rewrite sublist.length_concat.
-      rewrite shift_pairs_inner_length.
-      reflexivity. }
-    rewrite hlen. auto.
+    - rewrite shift_pairs_nil; cbn; auto.
+    - rewrite shift_pairs_cons; cbn.
+      pose proof IHh ess ltac:(auto) as ih; clear IHh.
+      assert (list_sum (map (length (A:=Exp.t)) (map snd ess))
+              = length (concat (snd (shift_pairs shift_exp ess)))) as hlen.
+      { unfold list_sum.
+        rewrite sublist.length_concat.
+        rewrite shift_pairs_inner_length.
+        reflexivity. }
+      rewrite hlen. auto.
   Qed.
 
   Polymorphic Lemma shift_pairs_relate_fst : forall es ess vs vss,
@@ -98,52 +97,53 @@ Section RelateExprDeclList.
       Forall2 (relate_decl_list R l) ess vss ->
       Forall2
         (R (concat vss ++ l))
-        (map fst (shift_pairs shift_exp (combine es ess))) vs.
+        (fst (shift_pairs shift_exp (combine es ess))) vs.
   Proof using A R l shift_exp_preserves_R.
     intros es ess vs vss hl hF3.
     generalize dependent ess.
     induction hF3; intros [| E ess] hl hF2;
       inv hF2; unravel in *; auto; try discriminate.
-    inv hl.
-    rewrite <- app_assoc.
-    rewrite map_snd_combine by assumption.
-    rewrite map_fst_map.
-    unfold list_sum.
-    rewrite <- sublist.length_concat.
-    assert (hlen : length (concat ess) = length (concat ts)).
-    { rewrite <- map_snd_combine with (us := us) (vs := ess)
-        in H5 by assumption.
-      apply shift_pairs_relate_snd in H5.
-      apply relate_decl_list_length in H5.
-      rewrite sublist.length_concat in H5 at 1.
-      rewrite shift_pairs_inner_length in H5.
-      rewrite <- sublist.length_concat in H5.
-      rewrite <- H5.
-      rewrite map_snd_combine by eauto.
-      reflexivity. }
-    rewrite hlen.
-    rewrite (relate_decl_list_length _ _ _ _ H3).
-    constructor; auto using shift_exp_preserves_R.
-    pose proof IHhF3 _ H1 H5 as ih; clear IHhF3.
-    clear dependent v.
-    clear dependent E.
-    clear dependent u.
-    clear hlen H5 hF3.
-    rewrite Forall2_forall_nth_error in *.
-    destruct ih as [hlen ih].
-    split.
-    - repeat rewrite map_length in *.
-      assumption.
-    - intros n e v he hv.
-      rewrite nth_error_map in he.
-      destruct (nth_error (map fst (shift_pairs shift_exp (combine us ess))) n)
-        as [se |] eqn:hse;
-        cbn in *;
-        try discriminate.
-      inv he.
-      pose proof ih _ _ _ hse hv as h.
-      pose proof shift_exp_preserves_R [] t0 _ _ _ h as H;
-        cbn in H.
-      assumption.
+    - rewrite shift_pairs_nil; cbn; auto.
+    - rewrite shift_pairs_cons; cbn; auto.
+      inv hl.
+      rewrite <- app_assoc.
+      rewrite map_snd_combine by assumption.
+      unfold list_sum.
+      rewrite <- sublist.length_concat.
+      assert (hlen : length (concat ess) = length (concat ts)).
+      { rewrite <- map_snd_combine with (us := us) (vs := ess)
+          in H5 by assumption.
+        apply shift_pairs_relate_snd in H5.
+        apply relate_decl_list_length in H5.
+        rewrite sublist.length_concat in H5 at 1.
+        rewrite shift_pairs_inner_length in H5.
+        rewrite <- sublist.length_concat in H5.
+        rewrite <- H5.
+        rewrite map_snd_combine by eauto.
+        reflexivity. }
+      rewrite hlen.
+      rewrite (relate_decl_list_length _ _ _ _ H3).
+      constructor; auto using shift_exp_preserves_R.
+      pose proof IHhF3 _ H1 H5 as ih; clear IHhF3.
+      clear dependent v.
+      clear dependent E.
+      clear dependent u.
+      clear hlen H5 hF3.
+      rewrite Forall2_forall_nth_error in *.
+      destruct ih as [hlen ih].
+      split.
+      +  repeat rewrite map_length in *.
+         assumption.
+      +  intros n e v he hv.
+         rewrite nth_error_map in he.
+         destruct (nth_error (fst (shift_pairs shift_exp (combine us ess))) n)
+           as [se |] eqn:hse;
+           cbn in *;
+           try discriminate.
+         inv he.
+         pose proof ih _ _ _ hse hv as h.
+         pose proof shift_exp_preserves_R [] t0 _ _ _ h as H;
+           cbn in H.
+         assumption.
   Qed.
 End RelateExprDeclList.
